Add lemmas relating compute up and down.

src/dafny/smart/synthattribute/ComputeRootPath.dfy
@@ -16,7 +16,7 @@ include "../intdiffalgo/DiffTree.dfy"
 include "../trees/CompleteTrees.dfy"
 include "GenericComputation.dfy"
 include "../helpers/Helpers.dfy"
-include "LeftSiblings.dfy"
+include "Siblings.dfy"
 include "../MerkleTrees.dfy"
 include "../paths/NextPathInCompleteTreesLemmas.dfy"
 include "../paths/PathInCompleteTrees.dfy"
@@ -30,7 +30,7 @@ module ComputeRootPath {
     import opened CompleteTrees
     import opened GenericComputation
     import opened Helpers
-    import opened LeftSiblings
+    import opened Siblings
     import opened MerkleTrees
     import opened NextPathInCompleteTreesLemmas
     import opened PathInCompleteTrees
@@ -38,107 +38,186 @@ module ComputeRootPath {
     import opened SeqHelpers
     import opened Trees
 
-    /**
-     *  Same as computeRootPath but uses default value 0 on 
-     *  right sibling to compute value at root.
-     *  Compute the value on a path recursively by computing on children first.
+    /**  
+     *  Compute the root value on a path bottom up.
+     *  
+     *  @param  p       A path.
+     *  @param  left    The value of `f` on each left sibling.
+     *  @param  right   The value of `f` on each right sibling.
+     *  @param  f       The binary operation to compute.
+     *  @param  seed    The value at the end of the path.
+     * 
      */
-    function method computeRootPathDiff(p : seq<bit>, b : seq<int>, seed: int) : int
-        requires |p| == |b|
+    function computeRootLeftRightUp<T>(p : seq<bit>, left : seq<T>, right: seq<T>, f : (T, T) -> T, seed: T) : T
+        requires |p| == |left| == |right|
         decreases p
     {
-        if |p| == 0 then 
-            seed
+        if |p| == 0 then
+            seed 
         else 
-            var r := computeRootPathDiff(tail(p), tail(b), seed);
-            if first(p) == 0 then
-                diff(r, 0)
-            else 
-                diff(first(b), r)
+            computeRootLeftRightUp(
+                init(p), init(left), init(right), f,
+                    if last(p) == 0 then f(seed, last(right)) else f(last(left), seed)
+            )
     }
 
     /**
-     *  Restrict computation to path of length >= 1.
+     *  Collect all the values on non-root node computed on the path p using left, right and seed.
+     *
+     *  @param  p       A path.
+     *  @param  left    The value of `f` on each left sibling.
+     *  @param  right   The value of `f` on each right sibling.
+     *  @param  f       The binary operation to compute.
+     *  @param  seed    The value at the end of the path.
      */
-     function computeRootPathDiff2(p : seq<bit>, b : seq<int>, seed: int) : int
-        requires |p| >= 1
-        requires |p| == |b|
-        ensures computeRootPathDiff2(p, b, seed) == computeRootPathDiff(p, b, seed)
+    function computeAllUp<T>(p : seq<bit>, left : seq<T>, right: seq<T>, f: (T, T) -> T, seed: T) : seq<T>
+        requires |p| == |left| == |right|
+        ensures |computeAllUp(p, left, right, f, seed)| == |p| 
         decreases p
     {
-        if |p| == 1 then 
-            computeRootPathDiff(p, b, seed)
+        if |p| == 0 then
+            [] 
         else 
-            var r := computeRootPathDiff(tail(p), tail(b), seed);
-            if first(p) == 0 then
-                diff(r, 0)
-            else 
-                diff(first(b), r)
+            // if last(p) == 0 then
+            //     computeAllUp(init(p), init(left), init(right), f, f(seed, last(right))) + [seed]
+            // else        
+            //     computeAllUp(init(p), init(left), init(right), f, f(last(left), seed)) + [seed]
+            computeAllUp(init(p), init(left), init(right), f,
+                 if last(p) == 0 then f(seed, last(right)) else f(last(left), seed)
+            ) 
+            + [seed]
     }
 
-    // lemma foo606(p : seq<bit>, b : seq<int>, seed: int)
-
     /**
-     *  Compute computeRootPathDiff by pre-computing the last 
-     *  step.
-     *  This corresponds to computing the value of the penultimate node on the path
-     *  and then use it to compute the value on the prefix path (without the last node).
+     *  Sub-lemma to split up computation of root on left/right sibings.
+     *
+     *  @param  p       A path.
+     *  @param  left    The value of `f` on each left sibling.
+     *  @param  right   The value of `f` on each right sibling.
+     *  @param  f       The binary operation to compute.
+     *  @param  seed    The value at the end of the path.
      */
-    lemma {:induction p, b} simplifyComputeRootPathDiffOnLast(p : seq<bit>, b : seq<int>, seed: int) 
-        requires 1 <= |p| == |b|
-        ensures computeRootPathDiff(p, b, seed) == 
-            computeRootPathDiff(
-                init(p), init(b), 
+    lemma {:induction p, left, right} simplifyComputeAll<T>(p : seq<bit>, left : seq<T>, right: seq<T>, f : (T, T) -> T, seed: T) 
+        requires 1 <= |p| == |left| == |right|
+        ensures computeAll(p, left, right, f, seed) == 
+            computeAll(
+                init(p), init(left), init(right), f, 
                 if last(p) == 0 then 
-                    diff(seed, 0)
+                    f(seed, last(right))
                 else 
-                    diff(last(b), seed)
-                )
+                    f(last(left), seed)
+                ) + [seed]
+        decreases p 
     {
         if |p| == 1 {
-            // Thanks Dafny
+            //  Thanks Dafny
         } else {
-            calc == {
-                init(tail(p));
-                { seqLemmas(p) ; }
-                tail(init(p));
-            }
-            calc == {
-                init(tail(b));
-                { seqLemmas(b) ; }
-                tail(init(b));
-            }
-            //  Dafny can work out the proof, with hint induction on tail(p), tail(b)
-            { simplifyComputeRootPathDiffOnLast(tail(p), tail(b), seed); }
-            if first(p) == 0 {
+            //  use the fact that init(tail(x)) == tail(init(x)) for p, left and right.
+            seqLemmas(p) ;
+            seqLemmas(left) ;
+            seqLemmas(right) ;
+            //  Dafny can work out the proof, with hint induction on tail(p), ...
+            simplifyComputeAll(tail(p), tail(left), tail(right), f, seed); 
+        }
+    }
+
+    /**
+     *  Collect all the values of the attribute on path p (including root).
+     * 
+     *  @param  p       A path.
+     *  @param  left    The value of `f` on each left sibling.
+     *  @param  right   The value of `f` on each right sibling.
+     *  @param  f       The binary operation to compute.
+     *  @param  seed    The value at the end of the path.
+     */
+    function computeAllUp2<T>(p : seq<bit>, left : seq<T>, right: seq<T>, f: (T, T) -> T, seed: T) : seq<T>
+        requires |p| == |left| == |right|
+        ensures |computeAllUp2(p, left, right, f, seed)| == |p| + 1
+        ensures computeAllUp2(p, left, right, f, seed)[0] == computeRootLeftRightUp(p, left, right, f, seed) == computeRootLeftRight(p, left, right, f, seed);
+        decreases p
+    {
+        computeLeftRightUpEqualsComputeLeftRight(p, left, right, f, seed);
+        if |p| == 0 then
+            [seed] 
+        else 
+            var newSeed := if last(p) == 0 then f(seed, last(right)) else f(last(left), seed);
+            computeAllUp2(init(p), init(left), init(right), f, newSeed) + [seed]
+    }
+
+
+    //  Properties of previous functions.
+
+    lemma {:induction p, left, right} computeAllUpEqualsComputeAll<T>(p : seq<bit>, left : seq<T>, right: seq<T>, f: (T, T) -> T, seed: T)
+        requires |p| == |left| == |right|
+        ensures computeAllUp2(p, left, right, f, seed) == computeAll(p, left, right, f, seed)
+    {
+        if |p| == 0 {
+            //  Thanks Dafny
+        } else {
+            if last(p) == 0 {
                 calc == {
-                    computeRootPathDiff(p, b, seed);
-                    diff(computeRootPathDiff(tail(p), tail(b), seed), 0);
-                    diff(
-                        computeRootPathDiff(init(tail(p)),init(tail(b)), 
-                            if last(p) == 0 then diff(seed, 0)
-                            else diff(last(b), seed)
-                        )
-                        , 0
-                    );
+                    computeAllUp2(p, left, right, f, seed);
+                    computeAllUp2(init(p), init(left), init(right), f, f(seed, last(right))) + [seed];
+                    //  Induction
+                    { computeAllUpEqualsComputeAll(init(p), init(left), init(right),  f, f(seed, last(right) ) )  ; }
+                    computeAll(init(p), init(left), init(right),  f, f(seed, last(right))) + [seed] ;
+                    { simplifyComputeAll(p, left, right, f, seed) ; }
+                    computeAll(p, left, right, f, seed);
+                }
+            } else {
+                calc == {
+                    computeAllUp2(p, left, right, f, seed);
+                    computeAllUp2(init(p), init(left), init(right), f, f(last(left), seed)) + [seed];
+                    //  Induction
+                    { computeAllUpEqualsComputeAll(init(p), init(left), init(right),  f, f(last(left), seed ) )  ; }
+                    computeAll(init(p), init(left), init(right),  f, f(last(left), seed)) + [seed] ;
+                    { simplifyComputeAll(p, left, right, f, seed) ; }
+                    computeAll(p, left, right, f, seed);
                 }
             }
-            else {  // first(p) == 1
+        }
+    }
+   
+    /**
+     *  Computing up or down yields same result.
+     */
+    lemma {:induction p, left, right, f} computeLeftRightUpEqualsComputeLeftRight<T>(p : seq<bit>, left : seq<T>, right: seq<T>, f : (T, T) -> T, seed: T)
+        requires |p| == |left| == |right|
+        ensures computeRootLeftRightUp(p, left, right, f, seed) == computeRootLeftRight(p, left, right, f, seed)
+        decreases p 
+    {
+        if |p| == 0 {
+            //  Thanks Dafny
+        } else {    
+            //  |p| >= 1
+            //  Split on values of last(p) 
+            if last(p) == 0 {
                 calc == {
-                    computeRootPathDiff(p, b, seed);
-                    diff(first(b), computeRootPathDiff(tail(p), tail(b), seed));
-                    diff(
-                        first(b),
-                        computeRootPathDiff(init(tail(p)), init(tail(b)), 
-                            if last(p) == 0 then diff(seed, 0)
-                            else diff(last(b), seed)
-                        )
-                    );
-                }            
+                    computeRootLeftRightUp(p, left, right, f, seed);
+                    computeRootLeftRightUp(init(p), init(left), init(right), f, f(seed, last(right)));
+                    //  Induction assumption
+                    { computeLeftRightUpEqualsComputeLeftRight(init(p), init(left), init(right), f, f(seed, last(right)));} 
+                    computeRootLeftRight(init(p), init(left), init(right), f, f(seed, last(right)));
+                    { simplifyComputeRootLeftRight(p, left, right, f, seed); }
+                    computeRootLeftRight(p, left, right, f, seed);
+                }
+            } else  {
+                calc == {
+                    computeRootLeftRightUp(p, left, right, f, seed);
+                    computeRootLeftRightUp(init(p), init(left), init(right), f, f(last(left), seed));
+                    //  Induction assumption
+                    { computeLeftRightUpEqualsComputeLeftRight(init(p), init(left), init(right), f, f(last(left), seed));} 
+                    computeRootLeftRight(init(p), init(left), init(right), f, f(last(left), seed));
+                    { simplifyComputeRootLeftRight(p, left, right, f, seed); }
+                    computeRootLeftRight(p, left, right, f, seed);
+                }
             }
         }
     }
 
+    /**
+     *  Sub-lemma to split up computation of root on left/right sibings.
+     */
     lemma {:induction p, left, right} simplifyComputeRootLeftRight<T>(p : seq<bit>, left : seq<T>, right: seq<T>, f : (T, T) -> T, seed: T) 
         requires 1 <= |p| == |left| == |right|
         ensures computeRootLeftRight(p, left, right, f, seed) == 
@@ -163,6 +242,233 @@ module ComputeRootPath {
         }
     }
 
+    lemma {:induction p, r, left, right} computeAllIsCorrectInATree<T>(p : seq<bit>, r : Tree<T>, left : seq<T>, right: seq<T>, f : (T, T) -> T, k : nat, seed: T, index : nat) 
+        requires isCompleteTree(r)
+        requires isDecoratedWith(f, r)
+        requires hasLeavesIndexedFrom(r, index)
+
+        requires k < |leavesIn(r)|
+        requires |p| == height(r) 
+        requires nodeAt(p, r) == leavesIn(r)[k]
+        requires seed == nodeAt(p,r).v 
+
+        requires |p| == |left| == |right|
+
+        /** Left and right contains siblings left and right values.  */
+        requires forall i :: 0 <= i < |p| ==>
+            siblingAt(take(p, i + 1), r).v == 
+                if p[i] == 0 then 
+                    right[i]
+                else 
+                    left[i]
+
+        ensures forall i :: 0 <= i <= |p| ==> 
+            nodeAt(take(p, i), r).v == computeAll(p, left, right, f, seed)[i]
+    {
+        forall (i : nat | 0 <= i <= |p|) 
+                ensures nodeAt(take(p, i), r).v == computeAll(p, left, right, f, seed)[i]
+        {
+            if |p| <= 1 {
+                //  Thanks Dafny
+            } else {
+                match r 
+                    case Node(_, lc, rc) => 
+                        completeTreeNumberLemmas(r);
+                        assert( |leavesIn(r)| == power2(height(r)));
+                        childrenCompTreeValidIndex(r, height(r), index);
+                        if ( i >= 1) {
+                            //  for i >= 1, induction on lc or rc depending on first(p)
+                            if first(p) == 0 {
+                                //  induction on lc
+                                //  Prove that pre-conditions on lc are satisfied
+                                childrenInCompTreesHaveSameNumberOfLeaves(r);
+                                assert(|leavesIn(lc)| == power2(height(r)) / 2);
+                                initPathDeterminesIndex(r, p, k, index);
+                                assert(k < power2(height(r)) / 2);
+                                assert(k < |leavesIn(lc)|);
+                                simplifyNodeAtFirstBit(p, r);
+                                assert(nodeAt(p, r) == nodeAt(tail(p), lc));
+                                assert(nodeAt(tail(p), lc).v == seed);
+
+                                projectLeftRightValuesOnChild(p, r, left, right);
+                                computeAllIsCorrectInATree(tail(p), lc, tail(left), tail(right), f, k, seed, index);
+
+                                // induction on lc
+                                assert(
+                                    forall k :: 0 <= k <= |tail(p)| ==> 
+                                        nodeAt(take(tail(p), k), lc).v == computeAll(tail(p), tail(left), tail(right), f, seed)[k]
+                                );
+
+                                //  R1:
+                                assert(nodeAt(take(tail(p), i - 1), lc).v == computeAll(tail(p), tail(left), tail(right), f, seed)[i - 1]);
+
+                                //  
+                                var x := computeAll(tail(p), tail(left), tail(right), f, seed);
+                                calc == {
+                                    computeAll(p, left, right, f, seed)[i];
+                                    ([ f(first(x), first(right))] + x)[i];
+                                    x[i - 1];
+                                    nodeAt(take(tail(p), i - 1), lc).v;
+                                    { simplifyNodeAtIndexFirstBit(p, r, i) ; }
+                                    nodeAt(take(p, i), r).v;
+                                }
+                            } else {
+                                //  induction on rc
+                                //  Prove that pre-conditions on lc are satisfied
+                                childrenInCompTreesHaveSameNumberOfLeaves(r);
+                                assert(|leavesIn(rc)| == power2(height(r)) / 2);
+                                initPathDeterminesIndex(r, p, k, index);
+                                assert(k >= power2(height(r)) / 2);
+                                var k' := k - power2(height(r)) / 2 ;
+                                assert(k' < |leavesIn(rc)|);
+                                simplifyNodeAtFirstBit(p, r);
+                                assert(nodeAt(p, r) == nodeAt(tail(p), rc));
+                                assert(nodeAt(tail(p), rc).v == seed);
+
+                                projectLeftRightValuesOnChild(p, r, left, right);
+                                computeAllIsCorrectInATree(tail(p), rc, tail(left), tail(right), f, k', seed, index + power2(height(r)) / 2);
+
+                                // induction on lc
+                                assert(
+                                    forall k :: 0 <= k <= |tail(p)| ==> 
+                                        nodeAt(take(tail(p), k), rc).v == computeAll(tail(p), tail(left), tail(right), f, seed)[k]
+                                );
+
+                                //  R1:
+                                assert(nodeAt(take(tail(p), i - 1), rc).v == computeAll(tail(p), tail(left), tail(right), f, seed)[i - 1]);
+
+                                //  
+                                var x := computeAll(tail(p), tail(left), tail(right), f, seed);
+                                calc == {
+                                    computeAll(p, left, right, f, seed)[i];
+                                    ([ f(first(left), first(x))] + x)[i];
+                                    x[i - 1];
+                                    nodeAt(take(tail(p), i - 1), rc).v;
+                                    { simplifyNodeAtIndexFirstBit(p, r, i) ; }
+                                    nodeAt(take(p, i), r).v;
+                                }
+                            }
+                        } else {    
+                            // i = 0, the node is the root
+                            calc == {
+                                nodeAt(take(p, 0), r).v;
+                                nodeAt([], r).v;
+                                r.v;
+                                { computeRootLeftRightIsCorrectForTree(p, r, left, right, f, seed) ; }
+                                computeRootLeftRight(p, left, right, f, seed);
+                                computeAllUp2(p, left, right, f, seed)[0];
+                                { computeAllUpEqualsComputeAll(p, left, right, f, seed); }
+                                computeAll(p, left, right, f, seed)[0];
+                            }
+                        }
+            }
+            
+        }
+    }
+
+    /**
+     *  Same as computeRootPath but uses default value 0 on 
+     *  right sibling to compute value at root.
+     *  Compute the value on a path recursively by computing on children first.
+     */
+    // function method computeRootPathDiff(p : seq<bit>, b : seq<int>, seed: int) : int
+    //     requires |p| == |b|
+    //     decreases p
+    // {
+    //     if |p| == 0 then 
+    //         seed
+    //     else 
+    //         var r := computeRootPathDiff(tail(p), tail(b), seed);
+    //         if first(p) == 0 then
+    //             diff(r, 0)
+    //         else 
+    //             diff(first(b), r)
+    // }
+
+    /**
+     *  Restrict computation to path of length >= 1.
+     */
+    //  function computeRootPathDiff2(p : seq<bit>, b : seq<int>, seed: int) : int
+    //     requires |p| >= 1
+    //     requires |p| == |b|
+    //     ensures computeRootPathDiff2(p, b, seed) == computeRootPathDiff(p, b, seed)
+    //     decreases p
+    // {
+    //     if |p| == 1 then 
+    //         computeRootPathDiff(p, b, seed)
+    //     else 
+    //         var r := computeRootPathDiff(tail(p), tail(b), seed);
+    //         if first(p) == 0 then
+    //             diff(r, 0)
+    //         else 
+    //             diff(first(b), r)
+    // }
+
+    // lemma foo606(p : seq<bit>, b : seq<int>, seed: int)
+
+    /**
+     *  Compute computeRootPathDiff by pre-computing the last 
+     *  step.
+     *  This corresponds to computing the value of the penultimate node on the path
+     *  and then use it to compute the value on the prefix path (without the last node).
+     */
+    // lemma {:induction p, b} simplifyComputeRootPathDiffOnLast(p : seq<bit>, b : seq<int>, seed: int) 
+    //     requires 1 <= |p| == |b|
+    //     ensures computeRootPathDiff(p, b, seed) == 
+    //         computeRootPathDiff(
+    //             init(p), init(b), 
+    //             if last(p) == 0 then 
+    //                 diff(seed, 0)
+    //             else 
+    //                 diff(last(b), seed)
+    //             )
+    // {
+    //     if |p| == 1 {
+    //         // Thanks Dafny
+    //     } else {
+    //         calc == {
+    //             init(tail(p));
+    //             { seqLemmas(p) ; }
+    //             tail(init(p));
+    //         }
+    //         calc == {
+    //             init(tail(b));
+    //             { seqLemmas(b) ; }
+    //             tail(init(b));
+    //         }
+    //         //  Dafny can work out the proof, with hint induction on tail(p), tail(b)
+    //         { simplifyComputeRootPathDiffOnLast(tail(p), tail(b), seed); }
+    //         if first(p) == 0 {
+    //             calc == {
+    //                 computeRootPathDiff(p, b, seed);
+    //                 diff(computeRootPathDiff(tail(p), tail(b), seed), 0);
+    //                 diff(
+    //                     computeRootPathDiff(init(tail(p)),init(tail(b)), 
+    //                         if last(p) == 0 then diff(seed, 0)
+    //                         else diff(last(b), seed)
+    //                     )
+    //                     , 0
+    //                 );
+    //             }
+    //         }
+    //         else {  // first(p) == 1
+    //             calc == {
+    //                 computeRootPathDiff(p, b, seed);
+    //                 diff(first(b), computeRootPathDiff(tail(p), tail(b), seed));
+    //                 diff(
+    //                     first(b),
+    //                     computeRootPathDiff(init(tail(p)), init(tail(b)), 
+    //                         if last(p) == 0 then diff(seed, 0)
+    //                         else diff(last(b), seed)
+    //                     )
+    //                 );
+    //             }            
+    //         }
+    //     }
+    // }
+
+  
+
     /**
      *  Compute root value starting from end of path.
      *  Recursive computation by simplifying the last step of the path i.e.
@@ -173,489 +479,420 @@ module ComputeRootPath {
      *  @param  seed    The new value to add at the end of p.
      *  @returns        The value of the root.
      */
-    function computeRootPathDiffUp(p : seq<bit>, b : seq<int>, seed: int) : int
-        requires |p| == |b|
-        decreases p
-    {
-     if |p| == 0 then
-        seed 
-    else 
-        if last(p) == 0 then
-            computeRootPathDiffUp(init(p), init(b),diff(seed, 0))
-        else        
-            computeRootPathDiffUp(init(p), init(b),diff(last(b), seed))
-    }
+    // function computeRootPathDiffUp(p : seq<bit>, b : seq<int>, seed: int) : int
+    //     requires |p| == |b|
+    //     decreases p
+    // {
+    //  if |p| == 0 then
+    //     seed 
+    // else 
+    //     if last(p) == 0 then
+    //         computeRootPathDiffUp(init(p), init(b),diff(seed, 0))
+    //     else        
+    //         computeRootPathDiffUp(init(p), init(b),diff(last(b), seed))
+    // }
 
-    /**  
-     *  Compute the root value bottom up.
-     *  @param  p       A path.
-     *  @param  left    The value of `f` on each left sibling.
-     *  @param  right   The value of `f` on each right sibling.
-     *  @param  f       The binary operation to compute.
-     *  @param  seed    The value at the end of the path.
-     * 
-     */
-    function computeRootLeftRightUp<T>(p : seq<bit>, left : seq<T>, right: seq<T>, f : (T, T) -> T, seed: T) : T
-        requires |p| == |left| == |right|
-        decreases p
-    {
-     if |p| == 0 then
-        seed 
-    else 
-        computeRootLeftRightUp(
-            init(p), init(left), init(right), f,
-            if last(p) == 0 then f(seed, last(right)) else f(last(left), seed)
-        )
-    }
+   
 
-    function computeRootPathDiffUp1(p : seq<bit>, b : seq<int>, seed: int) : int
-        requires 1 <= |p| == |b|
-        decreases p
-        ensures computeRootPathDiffUp1(p, b, seed) == computeRootPathDiffUp(p, b, seed)
-    {
-        if |p| == 1 then
-            if first(p) == 0 then diff(seed, 0) else diff(last(b), seed) 
-        else 
-            if last(p) == 0 then
-                computeRootPathDiffUp1(init(p), init(b),diff(seed, 0))
-            else        
-                computeRootPathDiffUp1(init(p), init(b),diff(last(b), seed))    
-    }
+    // function computeRootPathDiffUp1(p : seq<bit>, b : seq<int>, seed: int) : int
+    //     requires 1 <= |p| == |b|
+    //     decreases p
+    //     ensures computeRootPathDiffUp1(p, b, seed) == computeRootPathDiffUp(p, b, seed)
+    // {
+    //     if |p| == 1 then
+    //         if first(p) == 0 then diff(seed, 0) else diff(last(b), seed) 
+    //     else 
+    //         if last(p) == 0 then
+    //             computeRootPathDiffUp1(init(p), init(b),diff(seed, 0))
+    //         else        
+    //             computeRootPathDiffUp1(init(p), init(b),diff(last(b), seed))    
+    // }
 
     /**
      *  This version mixes the binary representation of a path and the corresponding
      *  positive integer k. It is used to prove that v3 is correct without
      *  having to do too much work.
      */
-    function computeRootPathDiffUpv2(p : seq<bit>, h: nat, k : nat, b : seq<int>, seed: int) : int
-        requires h == |p| == |b|
-        requires |p| >= 1
-        requires k < power2(|p|)
-        requires natToBitList(k, |p|) == p
-        ensures computeRootPathDiffUpv2(p, h, k, b, seed) == computeRootPathDiffUp(p, b, seed)
-        decreases p
-    {
-     if |p| == 1 then
-        if first(p) == 0 then diff(seed, 0)  else diff(last(b), seed)
-    else 
-        if last(p) == 0 then
-            assert( k % 2 == 0);
-            assert( h == |p|);
-            computeRootPathDiffUpv2(init(p), h - 1, k / 2, init(b),diff(seed, 0))
-        else        
-            assert( k % 2 == 1);
-            assert( h == |p|);
-            computeRootPathDiffUpv2(init(p), h - 1, k / 2, init(b),diff(last(b), seed))
-    }
+    // function computeRootPathDiffUpv2(p : seq<bit>, h: nat, k : nat, b : seq<int>, seed: int) : int
+    //     requires h == |p| == |b|
+    //     requires |p| >= 1
+    //     requires k < power2(|p|)
+    //     requires natToBitList(k, |p|) == p
+    //     ensures computeRootPathDiffUpv2(p, h, k, b, seed) == computeRootPathDiffUp(p, b, seed)
+    //     decreases p
+    // {
+    //  if |p| == 1 then
+    //     if first(p) == 0 then diff(seed, 0)  else diff(last(b), seed)
+    // else 
+    //     if last(p) == 0 then
+    //         assert( k % 2 == 0);
+    //         assert( h == |p|);
+    //         computeRootPathDiffUpv2(init(p), h - 1, k / 2, init(b),diff(seed, 0))
+    //     else        
+    //         assert( k % 2 == 1);
+    //         assert( h == |p|);
+    //         computeRootPathDiffUpv2(init(p), h - 1, k / 2, init(b),diff(last(b), seed))
+    // }
 
     /**
      *  Compute root value using the integer vaklue of a path.
      */
-    function method computeRootPathDiffUpv3(h: nat, k : nat, b : seq<int>, seed: int) : int
-        requires h == |b|
-        requires k < power2(h)
-        ensures  h >= 1 ==> 
-            computeRootPathDiffUpv3(h, k, b, seed) 
-                ==  var p := natToBitList(k, h);
-                    computeRootPathDiffUpv2(p, h, k, b, seed) 
-        decreases h
-    {
-    if h == 0 then
-        seed
-    else 
-        if k % 2 == 0 then
-            computeRootPathDiffUpv3(h - 1, k / 2, init(b),diff(seed, 0))
-        else        
-            computeRootPathDiffUpv3(h - 1, k / 2, init(b),diff(last(b), seed))
-    }
+    // function method computeRootPathDiffUpv3(h: nat, k : nat, b : seq<int>, seed: int) : int
+    //     requires h == |b|
+    //     requires k < power2(h)
+    //     ensures  h >= 1 ==> 
+    //         computeRootPathDiffUpv3(h, k, b, seed) 
+    //             ==  var p := natToBitList(k, h);
+    //                 computeRootPathDiffUpv2(p, h, k, b, seed) 
+    //     decreases h
+    // {
+    // if h == 0 then
+    //     seed
+    // else 
+    //     if k % 2 == 0 then
+    //         computeRootPathDiffUpv3(h - 1, k / 2, init(b),diff(seed, 0))
+    //     else        
+    //         computeRootPathDiffUpv3(h - 1, k / 2, init(b),diff(last(b), seed))
+    // }
 
-    lemma v3computesRootPath(h: nat, k : nat, b : seq<int>, seed: int) 
-        requires 1 <= h == |b|
-        requires k < power2(h)
-        ensures computeRootPathDiffUpv3(h, k, b, seed) == 
-            var p := natToBitList(k, h); computeRootPathDiffUpv2(p, h, k, b, seed) 
-        ensures computeRootPathDiffUpv3(h, k, b, seed) == 
-            var p := natToBitList(k, h); computeRootPathDiffUp(p, b, seed) 
-    {
-        //  Thanks Dafny
-    }
+    // lemma v3computesRootPath(h: nat, k : nat, b : seq<int>, seed: int) 
+    //     requires 1 <= h == |b|
+    //     requires k < power2(h)
+    //     ensures computeRootPathDiffUpv3(h, k, b, seed) == 
+    //         var p := natToBitList(k, h); computeRootPathDiffUpv2(p, h, k, b, seed) 
+    //     ensures computeRootPathDiffUpv3(h, k, b, seed) == 
+    //         var p := natToBitList(k, h); computeRootPathDiffUp(p, b, seed) 
+    // {
+    //     //  Thanks Dafny
+    // }
 
 
-    /**
-     *  Collect all the diff values computed on the path p.
-     */
-    function computeAllPathDiffUp(p : seq<bit>, b : seq<int>, seed: int) : seq<int>
-        requires |p| == |b|
-        ensures |computeAllPathDiffUp(p, b, seed)| == |p| 
-        decreases p
-    {
-     if |p| == 0 then
-        [] 
-    else 
-        if last(p) == 0 then
-            computeAllPathDiffUp(init(p), init(b), diff(seed, 0)) + [seed]
-        else        
-            computeAllPathDiffUp(init(p), init(b), diff(last(b), seed)) + [seed]
-    }
+   
 
     /**
      *  The sequence collected by computeAllPathDiffUp corresponds to the sequence
      *  of values computed by computeRootPathDiffUp on suffixes.
      */
-    lemma computeAllDiffUpPrefixes(p : seq<bit>, b : seq<int>, seed: int)
-        requires |p| == |b|
-        ensures forall i :: 0 <= i < |computeAllPathDiffUp(p, b, seed)| ==>
-            computeAllPathDiffUp(p, b, seed)[i] == computeRootPathDiffUp(drop(p, i + 1), drop(b, i + 1), seed) 
-    {
-        if |p| == 0 {
-            //  Thanks Dafny.
-        } else {
-            forall ( i : nat | 0 <= i < |p|)
-                ensures computeAllPathDiffUp(p, b, seed)[i] == computeRootPathDiffUp(drop(p, i + 1), drop(b, i + 1), seed) 
-            {
-                if last(p) == 0 {
-                    if i < |p| - 1 {
-                        calc == {
-                            computeRootPathDiffUp(p, b, seed);
-                            computeRootPathDiffUp(init(p), init(b), diff(seed, 0));
-                        }
-                        var a := computeAllPathDiffUp(init(p), init(b), diff(seed, 0)) + [diff(seed, 0)];
-                        calc == {
-                            computeAllPathDiffUp(p, b, seed)[i];
-                            a[i];
-                            { computeAllDiffUpPrefixes(init(p), init(b), diff(seed, 0)); }
-                            computeRootPathDiffUp(drop(init(p), i + 1), drop(init(b), i + 1), diff(seed, 0)); 
-                            calc == {   //  i + 1 < |p|
-                                init(drop(p, i + 1)) ; 
-                                { seqIndexLemmas(p, i + 1) ; }
-                                drop(init(p),i + 1);
-                            }   
-                            computeRootPathDiffUp(init(drop(p, i + 1)), init(b)[ i + 1..], diff(seed, 0));
-                            calc == { //  i + 1 < |p|
-                                init(drop(b, i + 1));
-                                { seqIndexLemmas(b, i + 1) ; }
-                                drop(init(b), i + 1);
-                            }  
-                            computeRootPathDiffUp(init(drop(p, i + 1)), init(drop(b, i + 1)), diff(seed, 0));
-                            //  Definition of computeRootPathDiffUp with last(p) == 0
-                            computeRootPathDiffUp(drop(p, i + 1), drop(b, i + 1), seed) ;
-                        }
-                    } else {
-                        //   i == |p| - 1
-                    }
-                } else {
-                    //  last(p) == 1, same as last(p) == 0 except that diff(seed, 0) is
-                    //  replaced by diff(last(b), seed)
-                    if i < |p| - 1 {
-                        calc == {
-                            computeRootPathDiffUp(p, b, seed);
-                            computeRootPathDiffUp(init(p), init(b), diff(last(b), seed));
-                        }
-                        var a := computeAllPathDiffUp(init(p), init(b), diff(last(b), seed)) + [diff(last(b), seed)];
-                        calc == {
-                            computeAllPathDiffUp(p, b, seed)[i];
-                            a[i];
-                            { computeAllDiffUpPrefixes(init(p), init(b), diff(last(b), seed)); }
-                            computeRootPathDiffUp(drop(init(p), i + 1), drop(init(b), i + 1), diff(last(b), seed)); 
-                            calc == {   //  i + 1 < |p|
-                                init(drop(p, i + 1)) ; 
-                                { seqIndexLemmas(p, i + 1) ; }
-                                drop(init(p), i + 1);
-                            }    
-                            computeRootPathDiffUp(init(drop(p, i + 1)), drop(init(b), i + 1), diff(last(b), seed));
-                           calc == { //  i + 1 < |p|
-                                init(drop(b, i + 1));
-                                { seqIndexLemmas(b, i + 1) ; }
-                                drop(init(b), i + 1);
-                            }   
-                            computeRootPathDiffUp(init(drop(p, i + 1)), init(drop(b, i + 1)) ,diff(last(b), seed));
-                            //  definition of computeRootPathDiffUp for last(p) == 1
-                            computeRootPathDiffUp(drop(p, i + 1), drop(b, i + 1), seed) ;
-                        }
-                    } else {
-                        //   i == |p| - 1
-                    }
-                }
-            }
-        }
-    }
+    // lemma computeAllDiffUpPrefixes(p : seq<bit>, b : seq<int>, seed: int)
+    //     requires |p| == |b|
+    //     ensures forall i :: 0 <= i < |computeAllPathDiffUp(p, b, seed)| ==>
+    //         computeAllPathDiffUp(p, b, seed)[i] == computeRootPathDiffUp(drop(p, i + 1), drop(b, i + 1), seed) 
+    // {
+    //     if |p| == 0 {
+    //         //  Thanks Dafny.
+    //     } else {
+    //         forall ( i : nat | 0 <= i < |p|)
+    //             ensures computeAllPathDiffUp(p, b, seed)[i] == computeRootPathDiffUp(drop(p, i + 1), drop(b, i + 1), seed) 
+    //         {
+    //             if last(p) == 0 {
+    //                 if i < |p| - 1 {
+    //                     calc == {
+    //                         computeRootPathDiffUp(p, b, seed);
+    //                         computeRootPathDiffUp(init(p), init(b), diff(seed, 0));
+    //                     }
+    //                     var a := computeAllPathDiffUp(init(p), init(b), diff(seed, 0)) + [diff(seed, 0)];
+    //                     calc == {
+    //                         computeAllPathDiffUp(p, b, seed)[i];
+    //                         a[i];
+    //                         { computeAllDiffUpPrefixes(init(p), init(b), diff(seed, 0)); }
+    //                         computeRootPathDiffUp(drop(init(p), i + 1), drop(init(b), i + 1), diff(seed, 0)); 
+    //                         calc == {   //  i + 1 < |p|
+    //                             init(drop(p, i + 1)) ; 
+    //                             { seqIndexLemmas(p, i + 1) ; }
+    //                             drop(init(p),i + 1);
+    //                         }   
+    //                         computeRootPathDiffUp(init(drop(p, i + 1)), init(b)[ i + 1..], diff(seed, 0));
+    //                         calc == { //  i + 1 < |p|
+    //                             init(drop(b, i + 1));
+    //                             { seqIndexLemmas(b, i + 1) ; }
+    //                             drop(init(b), i + 1);
+    //                         }  
+    //                         computeRootPathDiffUp(init(drop(p, i + 1)), init(drop(b, i + 1)), diff(seed, 0));
+    //                         //  Definition of computeRootPathDiffUp with last(p) == 0
+    //                         computeRootPathDiffUp(drop(p, i + 1), drop(b, i + 1), seed) ;
+    //                     }
+    //                 } else {
+    //                     //   i == |p| - 1
+    //                 }
+    //             } else {
+    //                 //  last(p) == 1, same as last(p) == 0 except that diff(seed, 0) is
+    //                 //  replaced by diff(last(b), seed)
+    //                 if i < |p| - 1 {
+    //                     calc == {
+    //                         computeRootPathDiffUp(p, b, seed);
+    //                         computeRootPathDiffUp(init(p), init(b), diff(last(b), seed));
+    //                     }
+    //                     var a := computeAllPathDiffUp(init(p), init(b), diff(last(b), seed)) + [diff(last(b), seed)];
+    //                     calc == {
+    //                         computeAllPathDiffUp(p, b, seed)[i];
+    //                         a[i];
+    //                         { computeAllDiffUpPrefixes(init(p), init(b), diff(last(b), seed)); }
+    //                         computeRootPathDiffUp(drop(init(p), i + 1), drop(init(b), i + 1), diff(last(b), seed)); 
+    //                         calc == {   //  i + 1 < |p|
+    //                             init(drop(p, i + 1)) ; 
+    //                             { seqIndexLemmas(p, i + 1) ; }
+    //                             drop(init(p), i + 1);
+    //                         }    
+    //                         computeRootPathDiffUp(init(drop(p, i + 1)), drop(init(b), i + 1), diff(last(b), seed));
+    //                        calc == { //  i + 1 < |p|
+    //                             init(drop(b, i + 1));
+    //                             { seqIndexLemmas(b, i + 1) ; }
+    //                             drop(init(b), i + 1);
+    //                         }   
+    //                         computeRootPathDiffUp(init(drop(p, i + 1)), init(drop(b, i + 1)) ,diff(last(b), seed));
+    //                         //  definition of computeRootPathDiffUp for last(p) == 1
+    //                         computeRootPathDiffUp(drop(p, i + 1), drop(b, i + 1), seed) ;
+    //                     }
+    //                 } else {
+    //                     //   i == |p| - 1
+    //                 }
+    //             }
+    //         }
+    //     }
+    // }
 
     /**
      *  Computing up or down yield the same result!
      */
-    lemma {:induction p, b, seed} computeUpEqualsComputeDown(p : seq<bit>, b : seq<int>, seed: int) 
-        requires |p| == |b|
-        ensures computeRootPathDiffUp(p, b, seed) == computeRootPathDiff(p, b, seed)
-    {
-        if |p| <= 1 {
-            //  Thanks Dafny
-        } else {    
-            //  |p| >= 2
-            //  Split on values of last(p) 
-            if last(p) == 0 {
-                calc == {
-                    computeRootPathDiffUp(p, b, seed);
-                    computeRootPathDiffUp(init(p), init(b), diff(seed, 0));
-                    //  Induction assumption
-                    computeRootPathDiff(init(p), init(b), diff(seed, 0));
-                    { simplifyComputeRootPathDiffOnLast(p, b, seed); }
-                    computeRootPathDiff(p, b, seed);
-                }
-            } else  {
-                assert(last(p) == 1 );
-                calc == {
-                    computeRootPathDiffUp(p, b, seed);
-                     computeRootPathDiffUp(init(p), init(b), diff(last(b), seed));
-                    //  Induction assumption
-                    computeRootPathDiff(init(p), init(b),  diff(last(b), seed));
-                    { simplifyComputeRootPathDiffOnLast(p, b, seed); }
-                    computeRootPathDiff(p, b, seed);
-                }
-            }
-        }
-    }
+    // lemma {:induction p, b, seed} computeUpEqualsComputeDown(p : seq<bit>, b : seq<int>, seed: int) 
+    //     requires |p| == |b|
+    //     ensures computeRootPathDiffUp(p, b, seed) == computeRootPathDiff(p, b, seed)
+    // {
+    //     if |p| <= 1 {
+    //         //  Thanks Dafny
+    //     } else {    
+    //         //  |p| >= 2
+    //         //  Split on values of last(p) 
+    //         if last(p) == 0 {
+    //             calc == {
+    //                 computeRootPathDiffUp(p, b, seed);
+    //                 computeRootPathDiffUp(init(p), init(b), diff(seed, 0));
+    //                 //  Induction assumption
+    //                 computeRootPathDiff(init(p), init(b), diff(seed, 0));
+    //                 { simplifyComputeRootPathDiffOnLast(p, b, seed); }
+    //                 computeRootPathDiff(p, b, seed);
+    //             }
+    //         } else  {
+    //             assert(last(p) == 1 );
+    //             calc == {
+    //                 computeRootPathDiffUp(p, b, seed);
+    //                  computeRootPathDiffUp(init(p), init(b), diff(last(b), seed));
+    //                 //  Induction assumption
+    //                 computeRootPathDiff(init(p), init(b),  diff(last(b), seed));
+    //                 { simplifyComputeRootPathDiffOnLast(p, b, seed); }
+    //                 computeRootPathDiff(p, b, seed);
+    //             }
+    //         }
+    //     }
+    // }
 
-    lemma  computeLeftRightUpEqualsComputeLeftRight<T>(p : seq<bit>, left : seq<T>, right: seq<T>, f : (T, T) -> T, seed: T)
-        requires |p| == |left| == |right|
-        ensures computeRootLeftRightUp(p, left, right, f, seed) == computeRootLeftRight(p, left, right, f, seed)
-    {
-        if |p| == 0 {
-            //  Thanks Dafny
-        } else {    
-            //  |p| >= 1
-            //  Split on values of last(p) 
-            if last(p) == 0 {
-                calc == {
-                    computeRootLeftRightUp(p, left, right, f, seed);
-                    computeRootLeftRightUp(init(p), init(left), init(right), f, f(seed, last(right)));
-                    //  Induction assumption
-                    { computeLeftRightUpEqualsComputeLeftRight(init(p), init(left), init(right), f, f(seed, last(right)));} 
-                    computeRootLeftRight(init(p), init(left), init(right), f, f(seed, last(right)));
-                    { simplifyComputeRootLeftRight(p, left, right, f, seed); }
-                    computeRootLeftRight(p, left, right, f, seed);
-                }
-            } else  {
-                assume(
-                    computeRootLeftRightUp(p, left, right, f, seed) == computeRootLeftRight(p, left, right, f, seed)
-                );
-                // assert(last(p) == 1 );
-                // calc == {
-                //     computeRootPathDiffUp(p, b, seed);
-                //      computeRootPathDiffUp(init(p), init(b), diff(last(b), seed));
-                //     //  Induction assumption
-                //     computeRootPathDiff(init(p), init(b),  diff(last(b), seed));
-                //     { simplifyComputeRootPathDiffOnLast(p, b, seed); }
-                //     computeRootPathDiff(p, b, seed);
-                // }
-            }
-        }
-    }
+    
 
     /**
      *  Show that if right sibling values are zero,  computeRootPathDiff
      *  computes the same result as computeRootPath.
      */
-    lemma {:induction p} computeRootPathDiffEqualscomputeRootPath(p : seq<bit>, b : seq<int>, seed: int) 
-        requires |b| == |p| 
-        requires forall i :: 0 <= i < |b| ==> p[i] == 0 ==> b[i] == 0
-        ensures computeRootPathDiff(p, b, seed) == computeRootPath(p, b, diff, seed)
-        decreases p
-    {
-        if |p| == 0 {
-            //  Thanks Dafny
-        } else {
-            //  Compute result on suffixes tail(p), tail(b)
-            var r := computeRootPathDiff(tail(p), tail(b), seed);
-            var r' := computeRootPath(tail(p), tail(b), diff, seed);
+    // lemma {:induction p} computeRootPathDiffEqualscomputeRootPath(p : seq<bit>, b : seq<int>, seed: int) 
+    //     requires |b| == |p| 
+    //     requires forall i :: 0 <= i < |b| ==> p[i] == 0 ==> b[i] == 0
+    //     ensures computeRootPathDiff(p, b, seed) == computeRootPath(p, b, diff, seed)
+    //     decreases p
+    // {
+    //     if |p| == 0 {
+    //         //  Thanks Dafny
+    //     } else {
+    //         //  Compute result on suffixes tail(p), tail(b)
+    //         var r := computeRootPathDiff(tail(p), tail(b), seed);
+    //         var r' := computeRootPath(tail(p), tail(b), diff, seed);
 
-            //  Use inductive assumption on tail(p), tail(b) which implies r == r'
-            calc == {
-                r;
-                { computeRootPathDiffEqualscomputeRootPath(tail(p), tail(b), seed); }
-                r';
-            }
-            //  Finalise proof
-            calc == {   //  These terms are equal
-                computeRootPathDiff(p, b, seed) ;
-                if first(p) == 0 then diff(r, 0) else  diff(first(b), r);
-                if first(p) == 0 then diff(r', 0) else  diff(first(b), r');
-                computeRootPath(p, b, diff, seed);
-            }
-        }
-    }
+    //         //  Use inductive assumption on tail(p), tail(b) which implies r == r'
+    //         calc == {
+    //             r;
+    //             { computeRootPathDiffEqualscomputeRootPath(tail(p), tail(b), seed); }
+    //             r';
+    //         }
+    //         //  Finalise proof
+    //         calc == {   //  These terms are equal
+    //             computeRootPathDiff(p, b, seed) ;
+    //             if first(p) == 0 then diff(r, 0) else  diff(first(b), r);
+    //             if first(p) == 0 then diff(r', 0) else  diff(first(b), r');
+    //             computeRootPath(p, b, diff, seed);
+    //         }
+    //     }
+    // }
 
     /**
      *  When two vectors b and b' have the same values for i such that p[i] == 1,
      *  i.e. for every left sibling b and b' coincide, then 
      *  computeRootPathDiff(p, b, seed) == computeRootPathDiff(p, b', seed)
      */
-    lemma {:induction p} sameComputeDiffPath(p : seq<bit>, b : seq<int>, b': seq<int>, seed: int)
-        requires |b| == |p| == |b'|
-        requires forall i :: 0 <= i < |b| ==> p[i] == 1 ==> b[i] == b'[i]
-        ensures computeRootPathDiff(p, b, seed) == computeRootPathDiff(p, b', seed)
-        decreases p 
-    {
-        if |p| == 0 {
-            //
-        } else {
-            var r := computeRootPathDiff(tail(p), tail(b), seed);
-            var r' := computeRootPathDiff(tail(p), tail(b'), seed);
-            //  Use inductive assumption on tail(p), tail(b) which implies r == r'
-            calc == {
-                r;
-                { sameComputeDiffPath(tail(p), tail(b), tail(b'), seed); }
-                r';
-            }
-            //  Finalise proof
-            calc == {   //  These terms are equal
-                computeRootPathDiff(p, b, seed) ;
-                if first(p) == 0 then diff(r, 0) else  diff(first(b), r);
-                if first(p) == 0 then diff(r', 0) else  diff(first(b), r');
-                computeRootPathDiff(p, b', seed);
-            }
-        }
-    }
+    // lemma {:induction p} sameComputeDiffPath(p : seq<bit>, b : seq<int>, b': seq<int>, seed: int)
+    //     requires |b| == |p| == |b'|
+    //     requires forall i :: 0 <= i < |b| ==> p[i] == 1 ==> b[i] == b'[i]
+    //     ensures computeRootPathDiff(p, b, seed) == computeRootPathDiff(p, b', seed)
+    //     decreases p 
+    // {
+    //     if |p| == 0 {
+    //         //
+    //     } else {
+    //         var r := computeRootPathDiff(tail(p), tail(b), seed);
+    //         var r' := computeRootPathDiff(tail(p), tail(b'), seed);
+    //         //  Use inductive assumption on tail(p), tail(b) which implies r == r'
+    //         calc == {
+    //             r;
+    //             { sameComputeDiffPath(tail(p), tail(b), tail(b'), seed); }
+    //             r';
+    //         }
+    //         //  Finalise proof
+    //         calc == {   //  These terms are equal
+    //             computeRootPathDiff(p, b, seed) ;
+    //             if first(p) == 0 then diff(r, 0) else  diff(first(b), r);
+    //             if first(p) == 0 then diff(r', 0) else  diff(first(b), r');
+    //             computeRootPathDiff(p, b', seed);
+    //         }
+    //     }
+    // }
 
-    function makeB(p: seq<bit>, b: seq<int>) : seq<int> 
-        requires |p| == |b|
-        decreases p
-        ensures |makeB(p, b)| == |b| && forall i :: 0 <= i < |b| ==> if p[i] == 1 then makeB(p,b)[i] == b[i] else makeB(p, b)[i] == 0 
-    {
-        if |p| == 0 then
-            []
-        else    
-            [if first(p) == 0 then 0 else first(b)] + makeB(tail(p), tail(b))
-    }
+    // function makeB(p: seq<bit>, b: seq<int>) : seq<int> 
+    //     requires |p| == |b|
+    //     decreases p
+    //     ensures |makeB(p, b)| == |b| && forall i :: 0 <= i < |b| ==> if p[i] == 1 then makeB(p,b)[i] == b[i] else makeB(p, b)[i] == 0 
+    // {
+    //     if |p| == 0 then
+    //         []
+    //     else    
+    //         [if first(p) == 0 then 0 else first(b)] + makeB(tail(p), tail(b))
+    // }
 
     /**
      *  Weakening of computeOnPathYieldsRootValue, requesting values on left siblings only, when
      *  merkle tree and path is not last non-null leaf.
      */
-     lemma {:induction p, r, b} computeOnPathYieldsRootValueDiff(p : seq<bit>, r : Tree<int>, b : seq<int>, k : nat) 
+    //  lemma {:induction p, r, b} computeOnPathYieldsRootValueDiff(p : seq<bit>, r : Tree<int>, b : seq<int>, k : nat) 
 
-        requires isCompleteTree(r)
-        /** `r` is decorated with attribute `f`. */
-        requires isDecoratedWith(diff, r)
-        requires height(r) >= 1
+    //     requires isCompleteTree(r)
+    //     /** `r` is decorated with attribute `f`. */
+    //     requires isDecoratedWith(diff, r)
+    //     requires height(r) >= 1
 
-        /**  all leaves after the k leaf are zero. */
-        requires k < |leavesIn(r)|
-        requires forall i :: k < i < |leavesIn(r)| ==> leavesIn(r)[i].v == 0
+    //     /**  all leaves after the k leaf are zero. */
+    //     requires k < |leavesIn(r)|
+    //     requires forall i :: k < i < |leavesIn(r)| ==> leavesIn(r)[i].v == 0
 
-        /** p is the path to k leaf in r. */
-        requires hasLeavesIndexedFrom(r, 0)
-        requires |p| == height(r) 
-        requires nodeAt(p, r) == leavesIn(r)[k]
+    //     /** p is the path to k leaf in r. */
+    //     requires hasLeavesIndexedFrom(r, 0)
+    //     requires |p| == height(r) 
+    //     requires nodeAt(p, r) == leavesIn(r)[k]
 
-        requires |b| == |p|
-        /** `b` contains values at left siblings on path `p`. */
-        requires forall i :: 0 <= i < |b| ==> p[i] == 1 ==> b[i] == siblingAt(take(p, i + 1), r).v
+    //     requires |b| == |p|
+    //     /** `b` contains values at left siblings on path `p`. */
+    //     requires forall i :: 0 <= i < |b| ==> p[i] == 1 ==> b[i] == siblingAt(take(p, i + 1), r).v
 
-        ensures r.v == computeRootPathDiff(p, b, leavesIn(r)[k].v)
+    //     ensures r.v == computeRootPathDiff(p, b, leavesIn(r)[k].v)
 
-        decreases r
-    {
+    //     decreases r
+    // {
 
-        //  define a new seq b' that holds default values for right siblings
-        //  and prove that pre-conditions of computeOnPathYieldsRootValue hold.
-        var b' := makeB(p, b);
+    //     //  define a new seq b' that holds default values for right siblings
+    //     //  and prove that pre-conditions of computeOnPathYieldsRootValue hold.
+    //     var b' := makeB(p, b);
 
-        leavesRightOfNodeAtPathZeroImpliesRightSiblingsOnPathZero(r, k, p, 0);
-        assert(forall i :: 0 <= i < |p| ==> 
-            p[i] == 0 ==> siblingAt(take(p, i + 1), r).v == 0);
+    //     leavesRightOfNodeAtPathZeroImpliesRightSiblingsOnPathZero(r, k, p, 0);
+    //     assert(forall i :: 0 <= i < |p| ==> 
+    //         p[i] == 0 ==> siblingAt(take(p, i + 1), r).v == 0);
 
-        siblingsLeft(p, r, b, b', k, 0);
-        assert(forall i :: 0 <= i < |p| ==> b'[i] == siblingAt(take(p, i + 1), r).v);
+    //     siblingsLeft(p, r, b, b', k, 0);
+    //     assert(forall i :: 0 <= i < |p| ==> b'[i] == siblingAt(take(p, i + 1), r).v);
 
-        assert(forall i :: 0 <= i < |p| ==> p[i] == 0 ==> b'[i] == 0);
+    //     assert(forall i :: 0 <= i < |p| ==> p[i] == 0 ==> b'[i] == 0);
 
-        computeOnPathYieldsRootValue(p, r, b', diff, leavesIn(r)[k].v);
-        assert(computeRootPath(p, b', diff, leavesIn(r)[k].v) ==  r.v);
-        computeRootPathDiffEqualscomputeRootPath(p, b', leavesIn(r)[k].v);
-        assert(computeRootPathDiff(p, b',  leavesIn(r)[k].v) == computeRootPath(p, b', diff,  leavesIn(r)[k].v));
+    //     computeOnPathYieldsRootValue(p, r, b', diff, leavesIn(r)[k].v);
+    //     assert(computeRootPath(p, b', diff, leavesIn(r)[k].v) ==  r.v);
+    //     computeRootPathDiffEqualscomputeRootPath(p, b', leavesIn(r)[k].v);
+    //     assert(computeRootPathDiff(p, b',  leavesIn(r)[k].v) == computeRootPath(p, b', diff,  leavesIn(r)[k].v));
 
-        sameComputeDiffPath(p, b, b', leavesIn(r)[k].v);
-    }
+    //     sameComputeDiffPath(p, b, b', leavesIn(r)[k].v);
+    // }
 
     /**
      *  
      */
-    lemma {:induction p, r, b} computeOnPathYieldsRootValueDiff2(p : seq<bit>, r : Tree<int>, b : seq<int>, k : nat, index : nat) 
+    // lemma {:induction p, r, b} computeOnPathYieldsRootValueDiff2(p : seq<bit>, r : Tree<int>, b : seq<int>, k : nat, index : nat) 
 
-         requires isCompleteTree(r)
-        /** `r` is decorated with attribute `f`. */
-        requires isDecoratedWith(diff, r)
-        requires height(r) >= 1
+    //      requires isCompleteTree(r)
+    //     /** `r` is decorated with attribute `f`. */
+    //     requires isDecoratedWith(diff, r)
+    //     requires height(r) >= 1
 
-        /**  all leaves after the k leaf are zero. */
-        requires k < |leavesIn(r)|
-        requires forall i :: k < i < |leavesIn(r)| ==> leavesIn(r)[i].v == 0
+    //     /**  all leaves after the k leaf are zero. */
+    //     requires k < |leavesIn(r)|
+    //     requires forall i :: k < i < |leavesIn(r)| ==> leavesIn(r)[i].v == 0
 
-        /** p is the path to k leaf in r. */
-        requires hasLeavesIndexedFrom(r, index)
-        requires |p| == height(r) 
-        requires nodeAt(p, r) == leavesIn(r)[k]
+    //     /** p is the path to k leaf in r. */
+    //     requires hasLeavesIndexedFrom(r, index)
+    //     requires |p| == height(r) 
+    //     requires nodeAt(p, r) == leavesIn(r)[k]
 
-        requires |b| == |p|
-        /** `b` contains values at left siblings on path `p`. */
-        requires forall i :: 0 <= i < |b| ==> p[i] == 1 ==> b[i] == siblingAt(take(p, i + 1), r).v
+    //     requires |b| == |p|
+    //     /** `b` contains values at left siblings on path `p`. */
+    //     requires forall i :: 0 <= i < |b| ==> p[i] == 1 ==> b[i] == siblingAt(take(p, i + 1), r).v
 
-        ensures r.v == computeRootPathDiff(p, b, leavesIn(r)[k].v)
+    //     ensures r.v == computeRootPathDiff(p, b, leavesIn(r)[k].v)
 
-        decreases r
-    {
+    //     decreases r
+    // {
 
-        //  define a new seq b' that holds default values for right siblings
-        //  and prove that pre-conditions of computeOnPathYieldsRootValue hold.
-        var b' := makeB(p, b);
+    //     //  define a new seq b' that holds default values for right siblings
+    //     //  and prove that pre-conditions of computeOnPathYieldsRootValue hold.
+    //     var b' := makeB(p, b);
 
-        leavesRightOfNodeAtPathZeroImpliesRightSiblingsOnPathZero(r, k, p, index);
-        assert(forall i :: 0 <= i < |p| ==> 
-            p[i] == 0 ==> siblingAt(take(p, i + 1), r).v == 0);
+    //     leavesRightOfNodeAtPathZeroImpliesRightSiblingsOnPathZero(r, k, p, index);
+    //     assert(forall i :: 0 <= i < |p| ==> 
+    //         p[i] == 0 ==> siblingAt(take(p, i + 1), r).v == 0);
 
-        siblingsLeft(p, r, b, b', k, index);
-        assert(forall i :: 0 <= i < |p| ==> b'[i] == siblingAt(take(p, i + 1), r).v);
+    //     siblingsLeft(p, r, b, b', k, index);
+    //     assert(forall i :: 0 <= i < |p| ==> b'[i] == siblingAt(take(p, i + 1), r).v);
 
-        assert(forall i :: 0 <= i < |p| ==> p[i] == 0 ==> b'[i] == 0);
+    //     assert(forall i :: 0 <= i < |p| ==> p[i] == 0 ==> b'[i] == 0);
 
-        computeOnPathYieldsRootValue(p, r, b', diff, leavesIn(r)[k].v);
-        assert(computeRootPath(p, b', diff, leavesIn(r)[k].v) ==  r.v);
-        computeRootPathDiffEqualscomputeRootPath(p, b', leavesIn(r)[k].v);
-        assert(computeRootPathDiff(p, b',  leavesIn(r)[k].v) == computeRootPath(p, b', diff,  leavesIn(r)[k].v));
+    //     computeOnPathYieldsRootValue(p, r, b', diff, leavesIn(r)[k].v);
+    //     assert(computeRootPath(p, b', diff, leavesIn(r)[k].v) ==  r.v);
+    //     computeRootPathDiffEqualscomputeRootPath(p, b', leavesIn(r)[k].v);
+    //     assert(computeRootPathDiff(p, b',  leavesIn(r)[k].v) == computeRootPath(p, b', diff,  leavesIn(r)[k].v));
 
-        sameComputeDiffPath(p, b, b', leavesIn(r)[k].v);
-    }
+    //     sameComputeDiffPath(p, b, b', leavesIn(r)[k].v);
+    // }
 
     /**
      *  Main function to compute the root value.
      */
-     function computeRootDiffUp(p : seq<bit>, r : Tree<int>, b : seq<int>, k : nat) : int
-        requires isCompleteTree(r)
-        /** `r` is decorated with attribute `f`. */
-        requires isDecoratedWith(diff, r)
-        requires height(r) >= 1
+    //  function computeRootDiffUp(p : seq<bit>, r : Tree<int>, b : seq<int>, k : nat) : int
+    //     requires isCompleteTree(r)
+    //     /** `r` is decorated with attribute `f`. */
+    //     requires isDecoratedWith(diff, r)
+    //     requires height(r) >= 1
 
-        /**  all leaves after the k leaf are zero. */
-        requires k < |leavesIn(r)|
-        requires forall i :: k < i < |leavesIn(r)| ==> leavesIn(r)[i].v == 0
+    //     /**  all leaves after the k leaf are zero. */
+    //     requires k < |leavesIn(r)|
+    //     requires forall i :: k < i < |leavesIn(r)| ==> leavesIn(r)[i].v == 0
 
-        /** p is the path to k leaf in r. */
-        requires hasLeavesIndexedFrom(r, 0)
-        requires |p| == height(r) 
-        requires nodeAt(p, r) == leavesIn(r)[k]
+    //     /** p is the path to k leaf in r. */
+    //     requires hasLeavesIndexedFrom(r, 0)
+    //     requires |p| == height(r) 
+    //     requires nodeAt(p, r) == leavesIn(r)[k]
 
-        requires |b| == |p|
-        /** `b` contains values at left siblings on path `p`. */
-        requires forall i :: 0 <= i < |b| ==> p[i] == 1 ==> b[i] == siblingAt(take(p, i + 1), r).v
+    //     requires |b| == |p|
+    //     /** `b` contains values at left siblings on path `p`. */
+    //     requires forall i :: 0 <= i < |b| ==> p[i] == 1 ==> b[i] == siblingAt(take(p, i + 1), r).v
 
-        ensures r.v == computeRootDiffUp(p, r, b, k)
-    {
-        //  Values on left sibling are enough to compuute r.v using computeRootPathDiff
-        computeOnPathYieldsRootValueDiff(p, r, b, k);
-        //  Compute computeRootUp yields same value as computeRootPathDiff
-        computeUpEqualsComputeDown(p, b, leavesIn(r)[k].v);
-        computeRootPathDiffUp(p, b, leavesIn(r)[k].v)
-    }
+    //     ensures r.v == computeRootDiffUp(p, r, b, k)
+    // {
+    //     //  Values on left sibling are enough to compuute r.v using computeRootPathDiff
+    //     computeOnPathYieldsRootValueDiff(p, r, b, k);
+    //     //  Compute computeRootUp yields same value as computeRootPathDiff
+    //     computeUpEqualsComputeDown(p, b, leavesIn(r)[k].v);
+    //     computeRootPathDiffUp(p, b, leavesIn(r)[k].v)
+    // }
 
     /**
      *  Same as computeRootDiffUp but with simplified pre-conditions.
@@ -663,67 +900,67 @@ module ComputeRootPath {
      *      2.  conditions on the leaves of the tree are given by `l`
      *      3.  path is given by the integer value k
      */
-    function computeRootDiffUpMerkle(l: seq<int>, r : Tree<int>, b : seq<int>, k : nat) : int
-        requires height(r) >= 1
+    // function computeRootDiffUpMerkle(l: seq<int>, r : Tree<int>, b : seq<int>, k : nat) : int
+    //     requires height(r) >= 1
 
-        /** r is a Merkle tree for l. */
-        requires |l| == |leavesIn(r)|
-        requires isMerkle2(r, l, diff)
+    //     /** r is a Merkle tree for l. */
+    //     requires |l| == |leavesIn(r)|
+    //     requires isMerkle2(r, l, diff)
 
-        /**  All leaves after the k leaf in l are zero. */
-        requires k < power2(height(r))
-        requires forall i :: k < i < |l| ==> l[i] == 0
+    //     /**  All leaves after the k leaf in l are zero. */
+    //     requires k < power2(height(r))
+    //     requires forall i :: k < i < |l| ==> l[i] == 0
 
-        /** p is the path to k leaf in r. */
-        requires hasLeavesIndexedFrom(r, 0)
+    //     /** p is the path to k leaf in r. */
+    //     requires hasLeavesIndexedFrom(r, 0)
 
-        requires |b| == height(r) 
-        /** `b` contains values at left siblings on path `p`. */
-        requires 
-            var p := natToBitList2(k, height(r));
-            forall i :: 0 <= i < |b| ==> p[i] == 1 ==> b[i] == siblingAt(take(p, i + 1), r).v
+    //     requires |b| == height(r) 
+    //     /** `b` contains values at left siblings on path `p`. */
+    //     requires 
+    //         var p := natToBitList2(k, height(r));
+    //         forall i :: 0 <= i < |b| ==> p[i] == 1 ==> b[i] == siblingAt(take(p, i + 1), r).v
 
-        /** The result is the attribute value on the root of the tree. */
-        ensures r.v == computeRootDiffUpMerkle(l, r, b, k)
-    {
+    //     /** The result is the attribute value on the root of the tree. */
+    //     ensures r.v == computeRootDiffUpMerkle(l, r, b, k)
+    // {
 
-        /*  
-         *  To compute the result we build the path leading to k-th leaf and use
-         *  computeRootDiffUp.
-         */
+    //     /*  
+    //      *  To compute the result we build the path leading to k-th leaf and use
+    //      *  computeRootDiffUp.
+    //      */
 
-        //  Pre conditions for computeRootDiffUp
+    //     //  Pre conditions for computeRootDiffUp
 
-        //  requires k < |leavesIn(r)|
-        calc ==> {
-            true;
-            { completeTreeNumberLemmas(r); }
-            |leavesIn(r)| == power2(height(r) );
-            k < |leavesIn(r)|;
-        }
+    //     //  requires k < |leavesIn(r)|
+    //     calc ==> {
+    //         true;
+    //         { completeTreeNumberLemmas(r); }
+    //         |leavesIn(r)| == power2(height(r) );
+    //         k < |leavesIn(r)|;
+    //     }
 
-        //  requires forall i :: k < i < |leavesIn(r)| ==> leavesIn(r)[i].v == 0
-        calc ==> {
-            true;
-            { assert(isMerkle2(r, l, diff)) ; }
-            forall i :: 0 <= i < |l| ==> l[i] == leavesIn(r)[i].v;
-            { assert( forall i :: k < i < |l| ==> l[i] == 0) ; }
-            forall i :: k < i < |leavesIn(r)| ==> leavesIn(r)[i].v == 0;
-        }
+    //     //  requires forall i :: k < i < |leavesIn(r)| ==> leavesIn(r)[i].v == 0
+    //     calc ==> {
+    //         true;
+    //         { assert(isMerkle2(r, l, diff)) ; }
+    //         forall i :: 0 <= i < |l| ==> l[i] == leavesIn(r)[i].v;
+    //         { assert( forall i :: k < i < |l| ==> l[i] == 0) ; }
+    //         forall i :: k < i < |leavesIn(r)| ==> leavesIn(r)[i].v == 0;
+    //     }
 
-        var p := natToBitList2(k, height(r) );
+    //     var p := natToBitList2(k, height(r) );
 
-        //  requires nodeAt(p, r) == leavesIn(r)[k]
-        calc ==> {
-            p == natToBitList(k, height(r));
-            { bitToNatToBitsIsIdentity(k, height(r)); }
-            bitListToNat(p) == k;
-            { indexOfLeafisIntValueOfPath(p, r, k); }
-            nodeAt(p, r) == leavesIn(r)[k];
-        }
+    //     //  requires nodeAt(p, r) == leavesIn(r)[k]
+    //     calc ==> {
+    //         p == natToBitList(k, height(r));
+    //         { bitToNatToBitsIsIdentity(k, height(r)); }
+    //         bitListToNat(p) == k;
+    //         { indexOfLeafisIntValueOfPath(p, r, k); }
+    //         nodeAt(p, r) == leavesIn(r)[k];
+    //     }
 
-        computeRootDiffUp(p, r, b, k)
-    }
+    //     computeRootDiffUp(p, r, b, k)
+    // }
 
     /**
      *  A useful lemma need in the proof of v1Equalsv2 when |p| > 1 and last(p) == 1.
@@ -734,238 +971,238 @@ module ComputeRootPath {
      *
      *  @note   A tedious proof with lots of indices but not hard.
      */
-    lemma prefixOfComputation(p : seq<bit>, valOnLeftAt : seq<int>, seed: int, valOnPAt: seq<int>) 
-        requires |p| == |valOnLeftAt| ==  |valOnPAt|
-        requires |p| >= 2
-        requires forall i :: 0 <= i < |valOnPAt| ==> valOnPAt[i] == computeRootPathDiffUp(drop(p, i + 1), drop(valOnLeftAt, i + 1), seed) 
-        ensures last(p) == 1 ==> forall i :: 0 <= i < |init(valOnLeftAt)| ==> 
-                    init(valOnPAt)[i] == computeRootPathDiffUp(drop(init(p), i + 1), drop(init(valOnLeftAt), i + 1), diff(last(valOnLeftAt), seed)) 
-    {
-        if last(p) == 1 {
-            forall (i : nat  | 0 <= i < |init(valOnPAt)|)
-                    ensures init(valOnPAt)[i] == 
-                        computeRootPathDiffUp( 
-                            drop(init(p), i + 1), 
-                            drop(init(valOnLeftAt), i + 1), 
-                            diff(last(valOnLeftAt), seed)
-                        ) 
-            {
-                //  drop does not changes last element
-                calc == {
-                    last(drop(p, i + 1));
-                    { seqIndexLemmas(p, i + 1) ; }
-                    last(p);
-                    1;
-                }
-                //  as i < |init(valOnPAt)|, valOnPAt and init(valOnPAt) coincide
-                calc == {
-                    valOnPAt[i];
-                    { seqIndexLemmas(valOnPAt, i) ; }
-                    init(valOnPAt)[i];
-                }
-                calc == {
-                    computeRootPathDiffUp(
-                        drop(init(p), i + 1), 
-                        drop(init(valOnLeftAt), i + 1),
-                        diff(last(valOnLeftAt), seed) );
-                    { seqIndexLemmas(valOnLeftAt, i + 1);  seqIndexLemmas(p, i + 1);  }
-                    computeRootPathDiffUp(
-                                init(drop(p, i + 1)), 
-                                init(drop(valOnLeftAt, i + 1)),
-                                diff(last(valOnLeftAt), seed)) ;
-                    //  definition of computeRootPathDiffUp with last(drop(p, i + 1)) == 1
-                    computeRootPathDiffUp(drop(p, i + 1), drop(valOnLeftAt, i + 1),  diff(last(valOnLeftAt), diff(last(valOnLeftAt), seed))); 
-                    //  use requires
-                    valOnPAt[i];
-                    //  which is same s init(valOnPAt)[i]
-                }
-            }
-        }
-    }
+    // lemma prefixOfComputation(p : seq<bit>, valOnLeftAt : seq<int>, seed: int, valOnPAt: seq<int>) 
+    //     requires |p| == |valOnLeftAt| ==  |valOnPAt|
+    //     requires |p| >= 2
+    //     requires forall i :: 0 <= i < |valOnPAt| ==> valOnPAt[i] == computeRootPathDiffUp(drop(p, i + 1), drop(valOnLeftAt, i + 1), seed) 
+    //     ensures last(p) == 1 ==> forall i :: 0 <= i < |init(valOnLeftAt)| ==> 
+    //                 init(valOnPAt)[i] == computeRootPathDiffUp(drop(init(p), i + 1), drop(init(valOnLeftAt), i + 1), diff(last(valOnLeftAt), seed)) 
+    // {
+    //     if last(p) == 1 {
+    //         forall (i : nat  | 0 <= i < |init(valOnPAt)|)
+    //                 ensures init(valOnPAt)[i] == 
+    //                     computeRootPathDiffUp( 
+    //                         drop(init(p), i + 1), 
+    //                         drop(init(valOnLeftAt), i + 1), 
+    //                         diff(last(valOnLeftAt), seed)
+    //                     ) 
+    //         {
+    //             //  drop does not changes last element
+    //             calc == {
+    //                 last(drop(p, i + 1));
+    //                 { seqIndexLemmas(p, i + 1) ; }
+    //                 last(p);
+    //                 1;
+    //             }
+    //             //  as i < |init(valOnPAt)|, valOnPAt and init(valOnPAt) coincide
+    //             calc == {
+    //                 valOnPAt[i];
+    //                 { seqIndexLemmas(valOnPAt, i) ; }
+    //                 init(valOnPAt)[i];
+    //             }
+    //             calc == {
+    //                 computeRootPathDiffUp(
+    //                     drop(init(p), i + 1), 
+    //                     drop(init(valOnLeftAt), i + 1),
+    //                     diff(last(valOnLeftAt), seed) );
+    //                 { seqIndexLemmas(valOnLeftAt, i + 1);  seqIndexLemmas(p, i + 1);  }
+    //                 computeRootPathDiffUp(
+    //                             init(drop(p, i + 1)), 
+    //                             init(drop(valOnLeftAt, i + 1)),
+    //                             diff(last(valOnLeftAt), seed)) ;
+    //                 //  definition of computeRootPathDiffUp with last(drop(p, i + 1)) == 1
+    //                 computeRootPathDiffUp(drop(p, i + 1), drop(valOnLeftAt, i + 1),  diff(last(valOnLeftAt), diff(last(valOnLeftAt), seed))); 
+    //                 //  use requires
+    //                 valOnPAt[i];
+    //                 //  which is same s init(valOnPAt)[i]
+    //             }
+    //         }
+    //     }
+    // }
 
     /**
      *  This is the most tedious lemma to prove.
      *  Some simplifications may be welcome at some point.
      *  The verification time is also large and a timeout may occur (see it to a valeu >= 60sec).
      */
-    lemma computeAllPathDiffUpInATree(p : seq<bit>, r : Tree<int>, b : seq<int>, k : nat, seed: int, index : nat) 
-        requires isCompleteTree(r)
-        /** `r` is decorated with attribute `f`. */
-        requires isDecoratedWith(diff, r)
-        requires height(r) >= 1
+    // lemma computeAllPathDiffUpInATree(p : seq<bit>, r : Tree<int>, b : seq<int>, k : nat, seed: int, index : nat) 
+    //     requires isCompleteTree(r)
+    //     /** `r` is decorated with attribute `f`. */
+    //     requires isDecoratedWith(diff, r)
+    //     requires height(r) >= 1
 
-        /**  all leaves after the k leaf are zero. */
-        requires k < |leavesIn(r)|
-        requires forall i :: k < i < |leavesIn(r)| ==> leavesIn(r)[i].v == 0
+    //     /**  all leaves after the k leaf are zero. */
+    //     requires k < |leavesIn(r)|
+    //     requires forall i :: k < i < |leavesIn(r)| ==> leavesIn(r)[i].v == 0
 
-        /** p is the path to k leaf in r. */
-        requires hasLeavesIndexedFrom(r, index)
-        requires |p| == height(r) 
-        requires nodeAt(p, r) == leavesIn(r)[k]
-        requires seed == nodeAt(p,r).v 
+    //     /** p is the path to k leaf in r. */
+    //     requires hasLeavesIndexedFrom(r, index)
+    //     requires |p| == height(r) 
+    //     requires nodeAt(p, r) == leavesIn(r)[k]
+    //     requires seed == nodeAt(p,r).v 
 
-        requires |b| == |p|
-        /** `b` contains values at left siblings on path `p`. */
-        requires forall i :: 0 <= i < |b| ==> p[i] == 1 ==> b[i] == siblingAt(take(p, i + 1), r).v
+    //     requires |b| == |p|
+    //     /** `b` contains values at left siblings on path `p`. */
+    //     requires forall i :: 0 <= i < |b| ==> p[i] == 1 ==> b[i] == siblingAt(take(p, i + 1), r).v
 
-        ensures forall i :: 0 <= i < |p| ==> 
-            nodeAt(take(p, i + 1), r).v == computeAllPathDiffUp(p, b, seed)[i]
-    {
-        if |p| == 1 {
-            //  Thanks Dafny.
-        } else {
-            //  |p| >= 2
-            //  use induction to get i >=1 and computation on p[0] to get i == 0
-            forall ( i : nat |  0 <= i < |p| )
-                ensures nodeAt(take(p, i + 1), r).v == computeAllPathDiffUp(p, b, seed)[i]
-            {
-            match r 
-                case Node(_, lc, rc) => 
-                    var b':= makeB(p, b);
+    //     ensures forall i :: 0 <= i < |p| ==> 
+    //         nodeAt(take(p, i + 1), r).v == computeAllPathDiffUp(p, b, seed)[i]
+    // {
+    //     if |p| == 1 {
+    //         //  Thanks Dafny.
+    //     } else {
+    //         //  |p| >= 2
+    //         //  use induction to get i >=1 and computation on p[0] to get i == 0
+    //         forall ( i : nat |  0 <= i < |p| )
+    //             ensures nodeAt(take(p, i + 1), r).v == computeAllPathDiffUp(p, b, seed)[i]
+    //         {
+    //         match r 
+    //             case Node(_, lc, rc) => 
+    //                 var b':= makeB(p, b);
 
-                    //  Collect true facts
-                    calc ==> {
-                        true;
-                        isCompleteTree(r);
-                        height(lc) == height(rc) == height(r) - 1 &&
-                            isCompleteTree(lc) && isCompleteTree(rc);
-                    }
-                    calc ==> {
-                        true;
-                        { assert( isDecoratedWith(diff, r)) ; }
-                        isDecoratedWith(diff, lc) && isDecoratedWith(diff, rc);
-                    }
-                    calc ==> {
-                        true;
-                        { childrenCompTreeValidIndex(r, height(r), index); }
-                        hasLeavesIndexedFrom(lc, index) 
-                            && hasLeavesIndexedFrom(rc, index + power2(height(r))/ 2);
-                    }
-                    calc ==> {
-                        true;
-                        { childrenInCompTreesHaveHalfNumberOfLeaves(r, height(r)); }
-                        leavesIn(lc) == leavesIn(r)[.. power2(height(r)) / 2]
-                            && leavesIn(rc) == leavesIn(r)[power2(height(r)) / 2 ..];
-                    }
-                    calc ==> {
-                        true;
-                        { completeTreeNumberLemmas(r); }
-                         k < |leavesIn(r)| == power2(height(r));
-                    }
-                    calc ==> {
-                        true;
-                        { assert(forall i :: 0 <= i < |b| ==> p[i] == 1 ==> b[i] == siblingAt(take(p, i + 1), r).v) ;}
-                        forall i :: 0 <= i < |b| ==> p[i] == 1 ==> b[i] == siblingAt(take(p, i + 1), r).v;
-                        { siblingsLeft(p, r, b, b', k, index); }
-                        forall i :: 0 <= i < |b'| ==> b'[i] == siblingAt(take(p, i + 1), r).v;
-                    }
-                    calc ==> {
-                        true;
-                        { assert(forall i :: 0 <= i < |b| ==> p[i] == 1 ==> b[i] == siblingAt(take(p, i + 1), r).v) ;}
-                        forall i :: 0 <= i < |b| ==> p[i] == 1 ==> b[i] == siblingAt(take(p, i + 1), r).v;
-                        { projectValuesOnChild(p, r, b'); }
-                        forall k :: 0 <= k < |tail(b')|  ==>
-                            tail(b')[k] == siblingAt(take(tail(p), k + 1), if first(p) == 0 then lc else rc).v;
-                    }
+    //                 //  Collect true facts
+    //                 calc ==> {
+    //                     true;
+    //                     isCompleteTree(r);
+    //                     height(lc) == height(rc) == height(r) - 1 &&
+    //                         isCompleteTree(lc) && isCompleteTree(rc);
+    //                 }
+    //                 calc ==> {
+    //                     true;
+    //                     { assert( isDecoratedWith(diff, r)) ; }
+    //                     isDecoratedWith(diff, lc) && isDecoratedWith(diff, rc);
+    //                 }
+    //                 calc ==> {
+    //                     true;
+    //                     { childrenCompTreeValidIndex(r, height(r), index); }
+    //                     hasLeavesIndexedFrom(lc, index) 
+    //                         && hasLeavesIndexedFrom(rc, index + power2(height(r))/ 2);
+    //                 }
+    //                 calc ==> {
+    //                     true;
+    //                     { childrenInCompTreesHaveHalfNumberOfLeaves(r, height(r)); }
+    //                     leavesIn(lc) == leavesIn(r)[.. power2(height(r)) / 2]
+    //                         && leavesIn(rc) == leavesIn(r)[power2(height(r)) / 2 ..];
+    //                 }
+    //                 calc ==> {
+    //                     true;
+    //                     { completeTreeNumberLemmas(r); }
+    //                      k < |leavesIn(r)| == power2(height(r));
+    //                 }
+    //                 calc ==> {
+    //                     true;
+    //                     { assert(forall i :: 0 <= i < |b| ==> p[i] == 1 ==> b[i] == siblingAt(take(p, i + 1), r).v) ;}
+    //                     forall i :: 0 <= i < |b| ==> p[i] == 1 ==> b[i] == siblingAt(take(p, i + 1), r).v;
+    //                     { siblingsLeft(p, r, b, b', k, index); }
+    //                     forall i :: 0 <= i < |b'| ==> b'[i] == siblingAt(take(p, i + 1), r).v;
+    //                 }
+    //                 calc ==> {
+    //                     true;
+    //                     { assert(forall i :: 0 <= i < |b| ==> p[i] == 1 ==> b[i] == siblingAt(take(p, i + 1), r).v) ;}
+    //                     forall i :: 0 <= i < |b| ==> p[i] == 1 ==> b[i] == siblingAt(take(p, i + 1), r).v;
+    //                     { projectValuesOnChild(p, r, b'); }
+    //                     forall k :: 0 <= k < |tail(b')|  ==>
+    //                         tail(b')[k] == siblingAt(take(tail(p), k + 1), if first(p) == 0 then lc else rc).v;
+    //                 }
 
-                    if ( i >= 1 ) {
-                        if first(p) == 0 {
-                            calc ==> {
-                                first(p) == 0;
-                                { initPathDeterminesIndex(r, p, k, index); }
-                                 k < power2(height(r))/ 2;
-                            }
-                            calc == {
-                                nodeAt(take(p, i + 1), r).v;
-                                { 
-                                    foo777(p, r, i); 
-                                }
-                                nodeAt(take(tail(p), i), lc).v;
-                                { computeAllPathDiffUpInATree(tail(p), lc, tail(b'), k, seed, index); }
-                                computeAllPathDiffUp(tail(p), tail(b'), seed)[i - 1];
-                                { computeAllDiffUpPrefixes(tail(p), tail(b'), seed); }
-                                computeRootPathDiffUp(drop(p, i + 1), drop(b', i + 1), seed);
-                                { computeUpEqualsComputeDown(drop(p, i + 1), drop(b', i + 1), seed); }
-                                computeRootPathDiff(drop(p, i + 1), drop(b', i + 1), seed);
-                                { sameComputeDiffPath(drop(p, i + 1), drop(b', i + 1), drop(b, i + 1), seed); 
-                                }
-                                computeRootPathDiff(drop(p, i + 1), drop(b, i + 1), seed);
-                                { computeUpEqualsComputeDown(drop(p, i + 1), drop(b, i + 1), seed); 
-                                }
-                                computeRootPathDiffUp(drop(p, i + 1), drop(b, i + 1), seed);
-                                { computeAllDiffUpPrefixes(p, b, seed); }
-                                computeAllPathDiffUp(p, b, seed)[i];
-                            }
-                        } else {
-                            initPathDeterminesIndex(r, p, k, index);
-                            assert(k  >= power2(height(r))/ 2);
-                            var k' := k - power2(height(r))/ 2;
-                            var index' := index + power2(height(r))/ 2;
-                            calc == {
-                                nodeAt(take(p, i + 1), r).v;
-                                { 
-                                    foo777(p, r, i); 
-                                }
-                                nodeAt(take(tail(p), i), rc).v;
-                                { computeAllPathDiffUpInATree(tail(p), rc, tail(b'), k', seed, index'); }
-                                computeAllPathDiffUp(tail(p), tail(b'), seed)[i - 1];
-                                { computeAllDiffUpPrefixes(tail(p), tail(b'), seed); }
-                                computeRootPathDiffUp(drop(p, i + 1), drop(b', i + 1), seed);
-                                { computeUpEqualsComputeDown(drop(p, i + 1), drop(b', i + 1), seed); }
-                                computeRootPathDiff(drop(p, i + 1), drop(b', i + 1), seed);
-                                { sameComputeDiffPath(drop(p, i + 1), drop(b', i + 1), drop(b, i + 1), seed); 
-                                }
-                                computeRootPathDiff(drop(p, i + 1), drop(b, i + 1), seed);
-                                { computeUpEqualsComputeDown(drop(p, i + 1), drop(b, i + 1), seed); 
-                                }
-                                computeRootPathDiffUp(drop(p, i + 1), drop(b, i + 1), seed);
-                                { computeAllDiffUpPrefixes(p, b, seed); }
-                                computeAllPathDiffUp(p, b, seed)[i];
-                            }
-                        }
-                    } else {
-                        //  i == 0
-                        if first(p) == 0 {
-                            calc ==> {
-                                first(p) == 0;
-                                { initPathDeterminesIndex(r, p, k, index); }
-                                 k < power2(height(r))/ 2;
-                            }
-                            calc == {
-                                computeAllPathDiffUp(p, b, seed)[0];
-                                { computeAllDiffUpPrefixes(p, b, seed); }
-                                computeRootPathDiffUp(tail(p), tail(b),seed) ;
-                                { computeUpEqualsComputeDown(tail(p), tail(b), seed); }
-                                computeRootPathDiff(tail(p), tail(b),seed) ;
-                                { sameComputeDiffPath(tail(p), tail(b'), tail(b), seed); }
-                                computeRootPathDiff(tail(p), tail(b'), seed);
-                                { computeOnPathYieldsRootValueDiff2(tail(p), lc, tail(b'), k, index); }
-                                lc.v;
-                                nodeAt(take(p, 0 + 1), r).v;
-                            }
-                        } else {
-                           calc ==> {
-                                first(p) == 0;
-                                { initPathDeterminesIndex(r, p, k, index); }
-                                k >= power2(height(r))/ 2;
-                            }
-                            var k' := k - power2(height(r))/ 2;
-                            var index':= index + power2(height(r))/ 2;
-                            calc == {
-                                computeAllPathDiffUp(p, b, seed)[0];
-                                { computeAllDiffUpPrefixes(p, b, seed); }
-                                computeRootPathDiffUp(tail(p), tail(b),seed) ;
-                                { computeUpEqualsComputeDown(tail(p), tail(b), seed); }
-                                computeRootPathDiff(tail(p), tail(b),seed) ;
-                                { sameComputeDiffPath(tail(p), tail(b'), tail(b), seed); }
-                                computeRootPathDiff(tail(p), tail(b'), seed);
-                                { computeOnPathYieldsRootValueDiff2(tail(p), rc, tail(b'), k', index'); }
-                                rc.v;
-                                nodeAt(take(p, 0 + 1), r).v;
-                            }
-                        }
-                    }
-            }
-        }
-    }
+    //                 if ( i >= 1 ) {
+    //                     if first(p) == 0 {
+    //                         calc ==> {
+    //                             first(p) == 0;
+    //                             { initPathDeterminesIndex(r, p, k, index); }
+    //                              k < power2(height(r))/ 2;
+    //                         }
+    //                         calc == {
+    //                             nodeAt(take(p, i + 1), r).v;
+    //                             { 
+    //                                 foo777(p, r, i); 
+    //                             }
+    //                             nodeAt(take(tail(p), i), lc).v;
+    //                             { computeAllPathDiffUpInATree(tail(p), lc, tail(b'), k, seed, index); }
+    //                             computeAllPathDiffUp(tail(p), tail(b'), seed)[i - 1];
+    //                             { computeAllDiffUpPrefixes(tail(p), tail(b'), seed); }
+    //                             computeRootPathDiffUp(drop(p, i + 1), drop(b', i + 1), seed);
+    //                             { computeUpEqualsComputeDown(drop(p, i + 1), drop(b', i + 1), seed); }
+    //                             computeRootPathDiff(drop(p, i + 1), drop(b', i + 1), seed);
+    //                             { sameComputeDiffPath(drop(p, i + 1), drop(b', i + 1), drop(b, i + 1), seed); 
+    //                             }
+    //                             computeRootPathDiff(drop(p, i + 1), drop(b, i + 1), seed);
+    //                             { computeUpEqualsComputeDown(drop(p, i + 1), drop(b, i + 1), seed); 
+    //                             }
+    //                             computeRootPathDiffUp(drop(p, i + 1), drop(b, i + 1), seed);
+    //                             { computeAllDiffUpPrefixes(p, b, seed); }
+    //                             computeAllPathDiffUp(p, b, seed)[i];
+    //                         }
+    //                     } else {
+    //                         initPathDeterminesIndex(r, p, k, index);
+    //                         assert(k  >= power2(height(r))/ 2);
+    //                         var k' := k - power2(height(r))/ 2;
+    //                         var index' := index + power2(height(r))/ 2;
+    //                         calc == {
+    //                             nodeAt(take(p, i + 1), r).v;
+    //                             { 
+    //                                 foo777(p, r, i); 
+    //                             }
+    //                             nodeAt(take(tail(p), i), rc).v;
+    //                             { computeAllPathDiffUpInATree(tail(p), rc, tail(b'), k', seed, index'); }
+    //                             computeAllPathDiffUp(tail(p), tail(b'), seed)[i - 1];
+    //                             { computeAllDiffUpPrefixes(tail(p), tail(b'), seed); }
+    //                             computeRootPathDiffUp(drop(p, i + 1), drop(b', i + 1), seed);
+    //                             { computeUpEqualsComputeDown(drop(p, i + 1), drop(b', i + 1), seed); }
+    //                             computeRootPathDiff(drop(p, i + 1), drop(b', i + 1), seed);
+    //                             { sameComputeDiffPath(drop(p, i + 1), drop(b', i + 1), drop(b, i + 1), seed); 
+    //                             }
+    //                             computeRootPathDiff(drop(p, i + 1), drop(b, i + 1), seed);
+    //                             { computeUpEqualsComputeDown(drop(p, i + 1), drop(b, i + 1), seed); 
+    //                             }
+    //                             computeRootPathDiffUp(drop(p, i + 1), drop(b, i + 1), seed);
+    //                             { computeAllDiffUpPrefixes(p, b, seed); }
+    //                             computeAllPathDiffUp(p, b, seed)[i];
+    //                         }
+    //                     }
+    //                 } else {
+    //                     //  i == 0
+    //                     if first(p) == 0 {
+    //                         calc ==> {
+    //                             first(p) == 0;
+    //                             { initPathDeterminesIndex(r, p, k, index); }
+    //                              k < power2(height(r))/ 2;
+    //                         }
+    //                         calc == {
+    //                             computeAllPathDiffUp(p, b, seed)[0];
+    //                             { computeAllDiffUpPrefixes(p, b, seed); }
+    //                             computeRootPathDiffUp(tail(p), tail(b),seed) ;
+    //                             { computeUpEqualsComputeDown(tail(p), tail(b), seed); }
+    //                             computeRootPathDiff(tail(p), tail(b),seed) ;
+    //                             { sameComputeDiffPath(tail(p), tail(b'), tail(b), seed); }
+    //                             computeRootPathDiff(tail(p), tail(b'), seed);
+    //                             { computeOnPathYieldsRootValueDiff2(tail(p), lc, tail(b'), k, index); }
+    //                             lc.v;
+    //                             nodeAt(take(p, 0 + 1), r).v;
+    //                         }
+    //                     } else {
+    //                        calc ==> {
+    //                             first(p) == 0;
+    //                             { initPathDeterminesIndex(r, p, k, index); }
+    //                             k >= power2(height(r))/ 2;
+    //                         }
+    //                         var k' := k - power2(height(r))/ 2;
+    //                         var index':= index + power2(height(r))/ 2;
+    //                         calc == {
+    //                             computeAllPathDiffUp(p, b, seed)[0];
+    //                             { computeAllDiffUpPrefixes(p, b, seed); }
+    //                             computeRootPathDiffUp(tail(p), tail(b),seed) ;
+    //                             { computeUpEqualsComputeDown(tail(p), tail(b), seed); }
+    //                             computeRootPathDiff(tail(p), tail(b),seed) ;
+    //                             { sameComputeDiffPath(tail(p), tail(b'), tail(b), seed); }
+    //                             computeRootPathDiff(tail(p), tail(b'), seed);
+    //                             { computeOnPathYieldsRootValueDiff2(tail(p), rc, tail(b'), k', index'); }
+    //                             rc.v;
+    //                             nodeAt(take(p, 0 + 1), r).v;
+    //                         }
+    //                     }
+    //                 }
+    //         }
+    //     }
+    // }
  }
